remove unused exceptions

LLVM_DS_RBT/Extended_Assertion.thy
@@ -57,8 +57,7 @@ lemma rbt_of_reorient_empty [simp]:
 
 subsection \<open>Assertion\<close>
 
-datatype except =     
-  COLOR_EX | KEY_EX | VALUE_EX | PTO_EX
+datatype except = VALUE_EX
 
 fun assn_unless (infixl "unless" 40) where 
   "assn_unless assn b = (if b then \<box> else assn)"
@@ -83,10 +82,10 @@ fun rbt_assn_ext :: "('k, 'v, 'ki, 'vi) assn_tree \<Rightarrow> ('k \<times> exc
   "rbt_assn_ext ATEmpty ex p = \<up>(p = null)"
 | "rbt_assn_ext (ATBranch c k v ci li ki vi ri l r) ex p =
     (
-      \<upharpoonleft>ll_bpto (RBT_NODE ci li ki vi ri) p unless (k, PTO_EX) \<in> ex **
-      color_assn c ci unless (k, COLOR_EX) \<in> ex **
+      \<upharpoonleft>ll_bpto (RBT_NODE ci li ki vi ri) p **
+      color_assn c ci **
       rbt_assn_ext l ex li **
-      \<upharpoonleft>key_assn k ki unless (k, KEY_EX) \<in> ex **
+      \<upharpoonleft>key_assn k ki **
       \<upharpoonleft>value_assn v vi unless (k, VALUE_EX) \<in> ex **
       rbt_assn_ext r ex ri
     )"
@@ -95,7 +94,7 @@ lemmas rbt_assn_ext_unfold = rbt_assn_ext.simps(2)
 
 
 lemma rbt_assn_ext_null [simp]: 
-  "(\<And>k. (k, PTO_EX) \<notin> ex) \<Longrightarrow> rbt_assn_ext t ex null = \<up>(t =  ATEmpty)"
+  "rbt_assn_ext t ex null = \<up>(t =  ATEmpty)"
   apply (cases t)
   using rbt_assn_ext_unfold apply auto
   done
@@ -109,7 +108,6 @@ subsection \<open>Load Rules\<close>
 
 lemma load_rbt [vcg_rules]:
   "
-    (k, PTO_EX) \<notin> ex \<Longrightarrow>
     llvm_htriple
     (rbt_assn_ext (ATBranch c k v ci li ki vi ri l r) ex ti)
     (ll_load ti)
@@ -149,10 +147,10 @@ lemma unfold_rbt_assn_ext_red_rule_1 [fri_red_rules]:
     is_sep_red
     (\<upharpoonleft>ll_bpto (RBT_NODE ci li ki vi ri) ti)
     (
-        \<upharpoonleft>ll_bpto (RBT_NODE ci li ki vi ri) ti unless (k, PTO_EX) \<in> ex **
-        color_assn c ci unless (k, COLOR_EX) \<in> ex **
+        \<upharpoonleft>ll_bpto (RBT_NODE ci li ki vi ri) ti **
+        color_assn c ci **
         rbt_assn_ext l ex li **
-        \<upharpoonleft>key_assn k ki unless (k, KEY_EX) \<in> ex **
+        \<upharpoonleft>key_assn k ki **
         \<upharpoonleft>value_assn v vi unless (k, VALUE_EX) \<in> ex **
         rbt_assn_ext r ex ri
     )
@@ -169,10 +167,10 @@ lemma unfold_rbt_assn_ext_red_rule_2 [fri_red_rules]:
     is_sep_red
     (\<upharpoonleft>ll_bpto (RBT_NODE ci li ki vi ri) ti unless cond)
     (
-        \<upharpoonleft>ll_bpto (RBT_NODE ci li ki vi ri) ti unless (k, PTO_EX) \<in> ex **
-        color_assn c ci unless (k, COLOR_EX) \<in> ex **
+        \<upharpoonleft>ll_bpto (RBT_NODE ci li ki vi ri) ti **
+        color_assn c ci **
         rbt_assn_ext l ex li **
-        \<upharpoonleft>key_assn k ki unless (k, KEY_EX) \<in> ex **
+        \<upharpoonleft>key_assn k ki **
         \<upharpoonleft>value_assn v vi unless (k, VALUE_EX) \<in> ex **
         rbt_assn_ext r ex ri
     )
@@ -254,9 +252,9 @@ lemma rbt_assn_ext_left_assn_unfold [fri_red_rules]:
   "
     is_sep_red
     (
-      \<upharpoonleft>ll_bpto (RBT_NODE ci li ki vi ri) ti unless (k, PTO_EX) \<in> ex **
-      color_assn c ci unless (k, COLOR_EX) \<in> ex **
-      \<upharpoonleft>key_assn k ki unless (k, KEY_EX) \<in> ex **
+      \<upharpoonleft>ll_bpto (RBT_NODE ci li ki vi ri) ti **
+      color_assn c ci **
+      \<upharpoonleft>key_assn k ki **
       \<upharpoonleft>value_assn v vi unless (k, VALUE_EX) \<in> ex \<and>*
       rbt_assn_ext r ex ri)
     \<box>
@@ -275,10 +273,10 @@ lemma rbt_assn_ext_right_assn_unfold [fri_red_rules]:
   "
     is_sep_red
     (
-      \<upharpoonleft>ll_bpto (RBT_NODE ci li ki vi ri) ti unless (k, PTO_EX) \<in> ex **
-      color_assn c ci unless (k, COLOR_EX) \<in> ex **
+      \<upharpoonleft>ll_bpto (RBT_NODE ci li ki vi ri) ti **
+      color_assn c ci **
       rbt_assn_ext l ex li **
-      \<upharpoonleft>key_assn k ki unless (k, KEY_EX) \<in> ex **
+      \<upharpoonleft>key_assn k ki **
       \<upharpoonleft>value_assn v vi unless (k, VALUE_EX) \<in> ex
     )
     \<box>
