LLVM_DS_RBT/Lookup/Lookup_Extended_Assertion.thy
@@ -74,7 +74,7 @@ next
     apply vcg
     subgoal
       apply vcg_compat
-      apply sep
+      apply (sepwith simp) 
        apply (cases "rbt_lookup (rbt_of al) kn")
         apply (auto simp add: ptr_of_key.simps)
       apply (sepwith simp)
@@ -83,7 +83,7 @@ next
     apply vcg
     subgoal
       apply vcg_compat
-      apply sep
+      apply (sepwith simp)
       apply (cases "rbt_lookup (rbt_of ar) kn")
       apply (auto simp add: ptr_of_key.simps)
       apply (sepwith simp)
